progress in WCommit and invariants

txn-data-consistency/EP+_Invariants.thy
@@ -793,14 +793,14 @@ lemma kvs_writers_readers_disjoint:
   "reach tps_s s \<Longrightarrow> kvs_writers (kvs_of_s s) \<inter> Tn ` kvs_readers (kvs_of_s s) = {}" oops
 
 definition RO_has_rts where
-  "RO_has_rts s \<longleftrightarrow> (\<forall>t. Tn t \<in> read_only_Txs (kvs_of_s s) \<longrightarrow> (\<exists>rts. rtxn_rts s t = Some rts))" (* not proven *)
+  "RO_has_rts s \<longleftrightarrow> (\<forall>t. Tn t \<in> read_only_Txs (kvs_of_s s) \<longrightarrow> (\<exists>rts. rtxn_rts s t = Some rts))"
 
-definition SO_ROs where
-  "SO_ROs s \<longleftrightarrow> (\<forall>r1 r2 rts1 rts2. (Tn r1, Tn r2) \<in> SO \<and>
+definition SO_Rts_Mono where
+  "SO_Rts_Mono s \<longleftrightarrow> (\<forall>r1 r2 rts1 rts2. (Tn r1, Tn r2) \<in> SO \<and>
     rtxn_rts s r1 = Some rts1 \<and> rtxn_rts s r2 = Some rts2 \<longrightarrow> rts1 \<le> rts2)"
 
-definition SO_RO_WR where
-  "SO_RO_WR s \<longleftrightarrow> (\<forall>r w rts cts. (Tn r, w) \<in> SO \<and>
+definition SO_Rts_Cts_Mono where
+  "SO_Rts_Cts_Mono s \<longleftrightarrow> (\<forall>r w rts cts. (Tn r, w) \<in> SO \<and>
     rtxn_rts s r = Some rts \<and> wtxn_cts s w = Some cts \<longrightarrow> rts \<le> cts)" (* not proven: commit events *)
 
 
